BoC/History.lean
@@ -9,10 +9,65 @@ inductive Event where
 | Run (bid : BId)
 | Complete (bid : BId)
 
+@[simp]
+def is_spawn : Event → Prop
+| .Spawn _ => True
+| _ => False
+
+@[simp]
+def is_run : Event → Prop
+| .Run _ => True
+| _ => False
+
+@[simp]
+def is_complete : Event → Prop
+| .Complete _ => True
+| _ => False
+
+@[simp]
 def Event.fresh (n : Nat) : Event -> Prop
 | .Spawn m => m < n
 | .Run m => m < n
 | .Complete m => m < n
+
+@[simp]
+def Event.lt : Event -> Event -> Prop
+| .Spawn bid1, e2
+| .Run bid1, e2
+| .Complete bid1, e2 =>
+    match e2 with
+    | .Spawn bid2
+    | .Run bid2
+    | .Complete bid2 => bid1 < bid2
+
+@[simp]
+def Event.leq : Event -> Event -> Prop
+| .Spawn bid1, e2
+| .Run bid1, e2
+| .Complete bid1, e2 =>
+    match e2 with
+    | .Spawn bid2
+    | .Run bid2
+    | .Complete bid2 => bid1 ≤ bid2
+
+@[simp]
+instance EventLT : LT Event where
+  lt := Event.lt
+
+@[simp]
+instance EventLE : LE Event where
+  le := Event.leq
+
+theorem Event.leq_refl (e : Event) : e ≤ e :=
+  by
+    rcases e <;> simp
+
+theorem Event.lt_neq (e1 e2 : Event) :
+    e1 < e2 →
+    e1 ≠ e2 :=
+  by
+    intro h_lt
+    rcases e1 <;> rcases e2 <;> simp at h_lt <;> grind
 
 -- A history maps behavior IDs and cowns to the events they have been involved
 -- in. An empty event list means the behavior or cown has not been run/used yet.
@@ -24,6 +79,11 @@ structure History where
 @[reducible]
 def History.empty : History :=
   History.mk (fun _ => []) (fun _ => [])
+
+@[simp]
+def History.fresh (n : Nat) (h : History) : Prop :=
+  (∀bid, ∀e ∈ h.behaviors bid, e.fresh n) ∧
+  (∀c, ∀e ∈ h.cowns c, e.fresh n)
 
 @[simp]
 def History.add_behavior_event (h : History) (bid : BId) (e : Event) : History :=
@@ -48,60 +108,64 @@ def History.add_cown_event (h : History) (cowns : List Cown) (e : Event) : Histo
 notation H "[" bid "+=" e "]" => History.add_behavior_event H bid e
 notation H "[" cowns "+=" e "]" => History.add_cown_event H cowns e
 
-@[simp]
 def wf_behavior_history_tail (bid : BId) : List Event → Prop
 | [] => True
 | [.Complete bid'] => bid = bid'
-| .Spawn bid' :: es =>
-    bid ≠ bid' ∧ wf_behavior_history_tail bid es
 | _ => False
 
-@[simp]
+def wf_behavior_history_spawns (bid : BId) : List Event → Prop
+| [] => True
+| .Spawn bid' :: es =>
+    bid < bid' ∧
+    (∀e ∈ es, (.Spawn bid' < e)) ∧
+    wf_behavior_history_spawns bid es
+| _ => False
+
 def wf_behavior_history (bid : BId) : List Event → Prop
 | [] => True
 | .Run bid' :: es =>
     bid = bid' ∧
-    wf_behavior_history_tail bid es ∧
-    List.Pairwise (· ≠ ·) es
+    ∃spawns tail, es = spawns ++ tail ∧
+      wf_behavior_history_spawns bid spawns ∧
+      wf_behavior_history_tail bid tail
 | _ => False
 
-@[simp]
+-- TODO: Could use this instead
+inductive WfBehaviorHistory (bid : BId) : List Event → Prop where
+| Empty :
+    WfBehaviorHistory bid []
+| NonEmpty {spawns tail} :
+    wf_behavior_history_spawns bid spawns →
+    wf_behavior_history_tail bid tail →
+    WfBehaviorHistory bid (.Run bid :: spawns ++ tail)
+
 def wf_cown_history : List Event → Prop
 | [] => True
 | [.Run _] => True
 | .Run bid :: .Complete bid' :: es =>
     bid = bid' ∧ wf_cown_history es ∧
-    .Run bid ∉ es ∧ .Complete bid' ∉ es
+    ∀e ∈ es, (.Run bid < e)
 | _ => False
 
-@[simp]
 def unique_spawns (h : BId → List Event) : Prop :=
   ∀bid1 bid2 bid,
     bid1 ≠ bid2 →
     .Spawn bid ∈ h bid1 →
     .Spawn bid ∉ h bid2
 
-inductive CausalStep (H : History) : Event → Event → Prop where
-| Seq {es1 es2 e1 e2 bid} :
-    H.behaviors bid = es1 ++ [e1, e2] ++ es2 →
-    CausalStep H e1 e2
-| Spawn {bid1 bid2 es} :
-    .Spawn bid2 ∈ H.behaviors bid1 →
-    H.behaviors bid2 = .Run bid2 :: es →
-    CausalStep H (.Spawn bid2) (.Run bid2)
-
-notation H "⊢" e1 "≺" e2 => ((CausalStep H)*) e1 e2
-
+@[simp]
 def History.wf (H : History) : Prop :=
+  -- Behavior histories are well-formed
   (∀bid, wf_behavior_history bid (H.behaviors bid))
   ∧
+  -- Spawn events are unique across behaviors
   unique_spawns H.behaviors
   ∧
+  -- Cown histories are well-formed
   (∀c, wf_cown_history (H.cowns c))
   ∧
-  (∀c, List.Pairwise (H ⊢ · ≺ ·) (H.cowns c))
-  ∧
-  is_partial_order (H ⊢ · ≺ ·)
+  -- Every cown event corresponds to some behavior event
+  (∀c e, e ∈ H.cowns c → ∃bid, e ∈ H.behaviors bid)
 
 notation "⊢" H => History.wf H
 
@@ -128,36 +192,23 @@ private def cyclic_history : History :=
 example : ¬ (⊢ cyclic_history) :=
   by
     intros h_contra
-    rcases h_contra with ⟨h_bid, h_unique, h_cown, h_pairwise, h_po⟩
-    have h_01 : cyclic_history ⊢ .Run 0 ≺ .Spawn 1 := by
-      apply Relation.ReflTransGen.single
-      apply @CausalStep.Seq cyclic_history [] [] (.Run 0) (.Spawn 1) 0
-      simp [cyclic_history]
-    have h_10 : cyclic_history ⊢ .Spawn 1 ≺ .Run 0 := by
-      apply @Relation.ReflTransGen.head Event _ (.Spawn 1) (.Run 1) (.Run 0)
-      · apply @CausalStep.Spawn cyclic_history 0 1 [.Spawn 0] <;> simp [cyclic_history]
-      · apply @Relation.ReflTransGen.head Event _ (.Run 1) (.Spawn 0) (.Run 0)
-        · apply @CausalStep.Seq cyclic_history [] [] (.Run 1) (.Spawn 0) 1
-          simp [cyclic_history]
-        · apply Relation.ReflTransGen.single
-          apply @CausalStep.Spawn cyclic_history 1 0 [.Spawn 1] <;> simp [cyclic_history]
-    apply is_partial_order_is_acyclic h_po (.Run 0) (.Spawn 1)
-    grind
+    rcases h_contra with ⟨h_bid, h_unique, h_cown, h_corr⟩
+    rcases h_bid 1 with ⟨_, ⟨spawns, tail, h_eq, h_spawns, h_tail⟩⟩
+    cases spawns with
+    | nil =>
+      simp at h_eq
+      subst h_eq
+      simp [wf_behavior_history_tail] at h_tail
+    | cons e spawns' =>
+      simp at h_eq
+      rcases h_eq with ⟨h_spawn, h_spawns_eq, h_tail_eq⟩
+      subst h_spawn h_spawns_eq
+      simp [wf_behavior_history_spawns] at h_spawns
 
 theorem empty_history_wf :
   ⊢ History.empty :=
   by
-    simp [History.wf]
-    · apply is_partial_order.mk
-      · apply Relation.ReflTransGen.refl
-      · intro a b c h_ab h_bc
-        apply Relation.ReflTransGen.trans h_ab h_bc
-      · intro a b h_ab h_ba
-        simp [History.empty] at h_ab
-        cases h_ab with
-        | refl => rfl
-        | tail h_ab h_step =>
-          cases h_step <;> simp at *
+    simp [History.wf, wf_behavior_history, wf_cown_history, unique_spawns]
 
 theorem empty_history_complete :
     History.complete History.empty :=
@@ -178,11 +229,324 @@ theorem wf_cown_history_no_dup {es} :
       | Run bid =>
         cases e' with
         | Complete bid' =>
-          rcases h_wf with ⟨h_eq, h_wf_tail, h_nin1, h_nin2⟩
+          rcases h_wf with ⟨h_eq, h_wf_tail, h_lt⟩
           subst h_eq
           simp
-          grind
+          and_intros <;> try grind [Event.lt_neq]
+          introv h_in
+          have := h_lt a' h_in
+          introv contra
+          subst contra
+          simp at *
         | _ =>
         simp [wf_cown_history] at h_wf
       | _ =>
         simp [wf_cown_history] at h_wf
+
+theorem wf_history_spawn_fresh H {bid fresh : BId} :
+    (⊢ H) →
+    Event.Run bid ∈ H.behaviors bid →
+    History.fresh fresh H →
+    ⊢ (H[bid += Event.Spawn fresh]) :=
+  by
+    introv h_wf h_run h_fresh
+    simp [History.wf]
+    rcases h_wf with ⟨h_behaviors, h_unique, h_cowns, h_corr⟩
+    and_intros <;> try (solve | grind)
+    · intros bid'
+      by_cases h_eq : bid' = bid
+      · simp [h_eq]
+        sorry -- Lemma about wf_behavior_history
+      · simp [h_eq]
+        grind
+    · sorry -- Lemma about unique_spawns
+
+lemma wf_history_tail_no_run_any {bid es} :
+    wf_behavior_history_tail bid es →
+    ∀e ∈ es, ¬is_run e :=
+  by
+    introv h_tail h_in
+    cases es with
+    | nil =>
+      simp at h_in
+    | cons e es' =>
+      cases e with
+      | Spawn b =>
+        simp [wf_behavior_history_tail] at h_tail
+      | Run b =>
+        simp [wf_behavior_history_tail] at h_tail
+      | Complete b =>
+        simp [wf_behavior_history_tail] at h_tail
+        rcases es' <;> simp at h_tail
+        simp at h_in
+        subst h_in
+        simp
+
+lemma wf_history_tail_mem_inv {bid es} :
+    wf_behavior_history_tail bid es →
+    ∀e ∈ es, is_complete e :=
+  by
+    introv h_tail h_in
+    cases es with
+    | nil =>
+      simp at h_in
+    | cons e es' =>
+      cases e with
+      | Spawn b =>
+        simp [wf_behavior_history_tail] at h_tail
+      | Run b =>
+        simp [wf_behavior_history_tail] at h_tail
+      | Complete b =>
+        simp [wf_behavior_history_tail] at h_tail
+        rcases es' <;> simp at h_tail
+        simp at h_in
+        subst h_in
+        simp
+
+theorem wf_history_spawns_no_run {bid es} :
+    wf_behavior_history_spawns bid es →
+    ∀e ∈ es, ¬is_run e :=
+  by
+    introv h_spawns h_in
+    induction es with
+    | nil =>
+      simp at h_in
+    | cons e es' ih =>
+      simp at h_in
+      cases h_in with
+      | inl h_eq =>
+        subst h_eq
+        rcases e <;> simp [wf_behavior_history_spawns] at h_spawns ⊢
+      | inr h_in' =>
+        rcases e <;> simp [wf_behavior_history_spawns] at h_spawns ⊢
+        rcases h_spawns with ⟨h_lt, h_es_lt, h_spawns'⟩
+        apply ih <;> assumption
+
+theorem wf_history_spawns_mem_inv {bid es} :
+    wf_behavior_history_spawns bid es →
+    ∀e ∈ es, is_spawn e :=
+  by
+    introv h_spawns h_in
+    induction es with
+    | nil =>
+      simp at h_in
+    | cons e es' ih =>
+      simp at h_in
+      cases h_in with
+      | inl h_eq =>
+        subst h_eq
+        rcases e <;> simp [wf_behavior_history_spawns] at h_spawns ⊢
+      | inr h_in' =>
+        rcases e <;> simp [wf_behavior_history_spawns] at h_spawns ⊢
+        rcases h_spawns with ⟨h_lt, h_es_lt, h_spawns'⟩
+        apply ih <;> assumption
+
+theorem wf_behavior_history_pair_inv {bid es e1 e2} :
+    wf_behavior_history bid es ->
+    [e1, e2] <:+: es →
+    is_run e1 ∧ is_spawn e2 ∨
+    is_run e1 ∧ is_complete e2 ∨
+    is_spawn e1 ∧ is_spawn e2 ∨
+    is_spawn e1 ∧ is_complete e2 :=
+  by
+    intro h_wf h_infix
+    simp [List.IsInfix] at h_infix
+    rcases h_infix with ⟨init, tail, h_eq⟩
+    subst h_eq
+    simp [wf_behavior_history] at h_wf
+    cases init with
+    | nil =>
+      simp at h_wf
+      rcases e1 <;> simp at h_wf
+      rcases h_wf with ⟨h_bid, spawns, tail', h_split, h_spawns, h_tail⟩
+      cases spawns with
+      | nil =>
+        simp at h_split
+        subst h_split
+        simp [wf_behavior_history_tail] at h_tail
+        rcases e2 <;> simp at h_tail ⊢
+      | cons e spawns' =>
+        simp at h_split
+        rcases h_split with ⟨h_eq, h_spawns_eq, h_tail_eq⟩
+        subst h_eq
+        rcases e2 <;> simp [wf_behavior_history_spawns] at h_spawns ⊢
+    | cons e init' =>
+      rcases e <;> simp at h_wf
+      rcases h_wf with ⟨h_bid, spawns, tail', h_split, h_spawns, h_tail⟩
+      have h_no_run : ∀e ∈ spawns ++ tail', ¬is_run e := by
+        intro e
+        intro h_mem
+        rcases List.mem_append.mp h_mem with h_mem_spawns | h_mem_tail
+        · have h_is := wf_history_spawns_mem_inv h_spawns e h_mem_spawns
+          rcases e <;> simp at h_is ⊢
+        · have h_is := wf_history_tail_mem_inv h_tail e h_mem_tail
+          rcases e <;> simp at h_is ⊢
+      cases e1 with
+      | Spawn b1 =>
+        cases e2 with
+        | Spawn b2
+        | Complete b2 => simp
+        | Run b2 =>
+          have h_mem : .Run b2 ∈ spawns ++ tail' := by
+            have : .Run b2 ∈ init' ++ .Spawn b1 :: .Run b2 :: tail := by simp
+            simpa [h_split] using this
+          exfalso
+          apply h_no_run _ h_mem
+          simp
+      | Run b1 =>
+        have h_mem : .Run b1 ∈ spawns ++ tail' := by
+          have : .Run b1 ∈ init' ++ .Run b1 :: e2 :: tail := by simp
+          simpa [h_split] using this
+        exfalso
+        apply h_no_run _ h_mem
+        simp
+      | Complete b1 =>
+        have h_mem : .Complete b1 ∈ spawns := by
+          cases List.eq_nil_or_concat tail' with
+          | inl h_eq =>
+            subst h_eq
+            have : .Complete b1 ∈ init' ++ .Complete b1 :: e2 :: tail := by simp
+            simpa [h_split] using this
+          | inr h_ex =>
+            rcases h_ex with ⟨tail'', e, h_eq⟩
+            subst h_eq
+            simp [wf_behavior_history_tail] at h_tail
+            rcases tail'' with _ | ⟨e, tail''⟩ <;> simp at h_tail
+            have h_eq : spawns ++ [].concat e = spawns.concat e := by simp
+            rw [h_eq] at h_split
+            cases List.eq_nil_or_concat tail with
+            | inl h_eq =>
+              subst h_eq
+              have h_eq : init' ++ [Event.Complete b1, e2] =
+                          (init' ++ [Event.Complete b1]).concat e2 := by simp
+              rw [h_eq] at h_split
+              have h_eq := List.init_eq_of_concat_eq h_split
+              subst h_eq
+              simp
+            | inr h_ex =>
+              rcases h_ex with ⟨spawns', e', h_eq⟩
+              rw [h_eq] at h_split
+              have h_eq : init' ++ Event.Complete b1 :: e2 :: spawns'.concat e' =
+                          (init' ++ Event.Complete b1 :: e2 :: spawns').concat e' := by simp
+              rw [h_eq] at h_split
+              have h_eq := List.init_eq_of_concat_eq h_split
+              subst h_eq
+              simp
+        exfalso
+        have contra := wf_history_spawns_mem_inv h_spawns _ h_mem
+        simp at contra
+
+theorem wf_history_spawns_no_dup {bid es} :
+    wf_behavior_history_spawns bid es →
+    List.Pairwise (· ≠ ·) es :=
+  by
+    intro h_wf
+    induction es with
+    | nil =>
+      simp
+    | cons e es' ih =>
+      rcases e <;> simp [wf_behavior_history_spawns] at h_wf
+      rcases h_wf with ⟨h_lt, h_es_lt, h_spawns'⟩
+      simp
+      and_intros <;> grind
+
+theorem wf_behavior_history_no_dup {bid es} :
+    wf_behavior_history bid es →
+    List.Pairwise (· ≠ ·) es :=
+  by
+    intro h_wf
+    cases es with
+    | nil =>
+      simp
+    | cons e es' =>
+      cases e with
+      | Spawn bid'
+      | Complete bid' =>
+        simp [wf_behavior_history] at h_wf
+      | Run bid' =>
+        simp [wf_behavior_history] at h_wf
+        rcases h_wf with ⟨h_eq, init, tail, h_eq', h_spawns, h_tail⟩
+        subst h_eq
+        subst h_eq'
+        simp
+        and_intros
+        · introv h_or
+          cases h_or with
+          | inl h_in =>
+            have h_spawn := wf_history_spawns_mem_inv h_spawns _ h_in
+            rcases a' <;> simp at h_spawn ⊢
+          | inr h_in =>
+            have h_tail := wf_history_tail_mem_inv h_tail _ h_in
+            rcases a' <;> simp at h_tail ⊢
+        · cases tail with
+          | nil =>
+            simp
+            exact wf_history_spawns_no_dup h_spawns
+          | cons e tail' =>
+            rcases e <;> rcases tail' <;> simp [wf_behavior_history_tail] at h_tail
+            subst h_tail
+            refine List.pairwise_append.mpr ?_
+            and_intros <;> try simp
+            · exact wf_history_spawns_no_dup h_spawns
+            · introv h_in h_in'
+              subst h_in'
+              have h_spawn := wf_history_spawns_mem_inv h_spawns _ h_in
+              simp at h_spawn
+
+theorem wf_history_run_mem_inv {bid bid' es} :
+    wf_behavior_history bid es →
+    .Run bid' ∈ es →
+    bid = bid' :=
+  by
+    intro h_wf h_in
+    cases es with
+    | nil =>
+      simp at h_in
+    | cons e es' =>
+      cases e with
+      | Spawn b
+      | Complete b =>
+        simp [wf_behavior_history] at h_wf
+      | Run b =>
+        simp [wf_behavior_history] at h_wf
+        rcases h_wf with ⟨h_eq, init, tail, h_eq', h_spawns, h_tail⟩
+        subst h_eq
+        subst h_eq'
+        simp at h_in
+        rcases h_in with h_eq | h_in | h_in
+        · subst h_eq
+          simp
+        · have contra := wf_history_spawns_mem_inv h_spawns _ h_in
+          simp at contra
+        · have contra := wf_history_tail_mem_inv h_tail _ h_in
+          simp at contra
+
+theorem wf_history_complete_mem_inv {bid bid' es} :
+    wf_behavior_history bid es →
+    .Complete bid' ∈ es →
+    bid = bid' :=
+  by
+    intro h_wf h_in
+    cases es with
+    | nil =>
+      simp at h_in
+    | cons e es' =>
+      cases e with
+      | Spawn b
+      | Complete b =>
+        simp [wf_behavior_history] at h_wf
+      | Run b =>
+        simp [wf_behavior_history] at h_wf
+        rcases h_wf with ⟨h_eq, init, tail, h_eq', h_spawns, h_tail⟩
+        subst h_eq
+        subst h_eq'
+        simp at h_in
+        rcases h_in with h_in | h_in
+        · have contra := wf_history_spawns_mem_inv h_spawns _ h_in
+          simp at contra
+        · cases tail with
+          | nil =>
+            simp at h_in
+          | cons e tail' =>
+            rcases e <;> rcases tail' <;> simp [wf_behavior_history_tail] at h_tail
+            grind
